\documentclass[12pt]{article}
\begin{document}
$$\frac{\frac{\frac{\frac{\frac{A0 \cdot A1 - \sin(x) \cdot \cos(x) \cdot 0 + 0 \cdot 1 + 0 \cdot 4 + A2 + 0 \cdot \ln(x) \cdot \ln(x) \cdot 1 + 0 \cdot \ln(x) \cdot \ln(x) \cdot 1}{A3 \cdot A4} \cdot x - A5}{x \cdot x} \cdot x - \frac{A6}{x} \cdot 1}{x \cdot x} \cdot x - \frac{\frac{A7}{x}}{x} \cdot 1}{x \cdot x} \cdot x - \frac{\frac{\frac{A8}{x}}{x}}{x} \cdot 1}{x \cdot x} \cdot \sin(x) + 1 \cdot \cos(x) \cdot \frac{\frac{\frac{\frac{A9}{x}}{x}}{x}}{x} \cdot \cos(x) + 1 \cdot (-1) \cdot \sin(x) \cdot \frac{\frac{\frac{\frac{A10}{x}}{x}}{x}}{x} \cdot \sin(x)$$ \\  \\ 
A0 = $1 \cdot \cos(x) \cdot \cos(x) + 1 \cdot (-1) \cdot \sin(x) \cdot \sin(x)$ \\ 
A1 = $5 + 4 \cdot 1 + \ln(x) \cdot \ln(x) \cdot 1 \cdot 1$ \\ 
A2 = $1 \cdot \frac{1}{x} \cdot \ln(x) + 1 \cdot \frac{1}{x} \cdot \ln(x) \cdot 1$ \\ 
A3 = $5 + 4 \cdot 1 + \ln(x) \cdot \ln(x) \cdot 1 \cdot 1$ \\ 
A4 = $5 + 4 \cdot 1 + \ln(x) \cdot \ln(x) \cdot 1 \cdot 1$ \\ 
A5 = $\frac{\sin(x) \cdot \cos(x)}{5 + 4 \cdot 1 + \ln(x) \cdot \ln(x) \cdot 1 \cdot 1} \cdot 1$ \\ 
A6 = $\frac{\sin(x) \cdot \cos(x)}{5 + 4 \cdot 1 + \ln(x) \cdot \ln(x) \cdot 1 \cdot 1}$ \\ 
A7 = $\frac{\sin(x) \cdot \cos(x)}{5 + 4 \cdot 1 + \ln(x) \cdot \ln(x) \cdot 1 \cdot 1}$ \\ 
A8 = $\frac{\sin(x) \cdot \cos(x)}{5 + 4 \cdot 1 + \ln(x) \cdot \ln(x) \cdot 1 \cdot 1}$ \\ 
A9 = $\frac{\sin(x) \cdot \cos(x)}{5 + 4 \cdot 1 + \ln(x) \cdot \ln(x) \cdot 1 \cdot 1}$ \\ 
A10 = $\frac{\sin(x) \cdot \cos(x)}{5 + 4 \cdot 1 + \ln(x) \cdot \ln(x) \cdot 1 \cdot 1}$ \\ 
\end{document}
